[WIP] progress check

theories/check.v
@@ -1,6 +1,8 @@
 From mathcomp Require Import all_ssreflect.
 From det Require Import lang.
 From det Require Import tree tree_prop.
+From elpi.apps Require Import derive derive.std.
+From HB Require Import structures.
 
 (* TODO:
 A valid state for substitutions is mandatory?
@@ -11,11 +13,33 @@ Is it important that the substitution in the Or note, X is a function?
 *)
 
 Set Implicit Arguments.
-Inductive typecheck A :=
-  | ty_ok : A -> typecheck
-  | ty_err.
+
+Section tc.
+  Variable A : eqType.
+  Inductive typecheck :=
+    | ty_ok : A -> typecheck
+    | ty_err.
+
+  Definition eqb_tc (A B: typecheck) :=
+    match A, B with
+    | ty_ok A, ty_ok B => A == B
+    | ty_err, ty_err => true
+    | _, _ => false
+    end.
+
+  Lemma eqb_tcP: Equality.axiom eqb_tc.
+  Proof.
+    move=> /= [x|][y|]//=; try by constructor.
+    case:eqP => H; constructor; congruence.
+  Qed.
+
+  HB.instance Definition _ := hasDecEq.Build typecheck eqb_tcP.
+
+  Compute (erefl : ty_err == ty_err).
+End tc.
 
 Arguments ty_err {_}.
+Arguments ty_ok {_}.
 
 
 Lemma tm2RC_kp {t1 k} : 
@@ -42,116 +66,67 @@ Section has_cut.
   (* tells if A has a superficial cut *)
   Fixpoint has_cut A :=
     match A with
-    | CutS | Bot | Dead => true
-    | OK | CallS _ _ => false
-    | And A B0 B => has_cut A || (has_cut B0 && has_cut B)
-    | Or _ _ _ => is_ko A
+    | CutS => true
+    | OK | CallS _ _ | Bot | Dead => false
+    | And A _ B => 
+      (* here, B0 is useless. B0 is used if A is failed while backtracking,
+         but B0 is resumed inside or and its cut have no effect outside the
+         And A B0 B tree
+      *)
+      ((failed A == false) && (has_cut A || has_cut B))
+    | Or _ _ _ => false
     end.
-
-  Lemma has_cut_cut {B}: has_cut (cutr B).
-  Proof. 
-    elim: B => //=.
-    - move=> ?????; rewrite !is_ko_cutr//.
-    - by move=> A ->.
-  Qed.
-
-  Lemma is_ko_has_cut {A}: is_ko A -> has_cut A.
-  Proof. elim: A => //=; move=> A HA B0 _ B HB dA; rewrite HA//. Qed.
-
-  Lemma is_dead_has_cut {A}: is_dead A -> has_cut A.
-  Proof. move=> /is_dead_is_ko /is_ko_has_cut//. Qed.
-
-  Lemma has_cut_cutl {A}: has_cut A -> has_cut (cutl A).
-  Proof.
-    elim: A => //.
-      move=> A HA s B HB/=/andP[kA kB]; rewrite fun_if/= is_ko_cutr kA !is_ko_cutl// if_same//.
-    move=> A HA B0 HB0 B HB /=/orP[cA|/andP[cB0 cB]].
-      by rewrite fun_if/=HA//= has_cut_cut if_same.
-    by rewrite fun_if /= HB// !has_cut_cut orbT if_same.
-  Qed.
-
-  Lemma expand_has_cut {u A s}: 
-    has_cut A -> has_cut (get_tree (expand u s A)) \/ is_cutbrothers (expand u s A).
-  Proof.
-    elim: A s; try by move=> /=; auto.
-    - move=> A HA s1 B HB s /=/andP[kA kB].
-      case: ifP => dA.
-        rewrite (is_ko_expand _ kB)/=kA kB; auto.
-      rewrite (is_ko_expand _ kA)/=kA kB; auto.
-    - move=> A HA B0 _ B HB s /=/orP[].
-        move=> /(HA s); case: expand => [|||] C/= []//; auto => cC.
-        - by rewrite cC /=; left.
-        - by rewrite cC /=; left.
-        left; rewrite get_tree_And /=.
-        by case: ifP; rewrite ?cC // has_cut_cutl.
-      case/andP=> cB0 cB.
-      case: expand => [|||] C/=; rewrite ?cB ?cB0 ?orbT; auto.
-      move: (HB (get_substS s C) cB).
-      by case: expand => [|||] D /=; auto => -[]// ->; rewrite cB0 orbT; left.
-  Qed.
 
   Lemma has_cut_success {A}:
     has_cut A -> success A = false.
   Proof.
     elim: A => //.
-    - move=> A HA s B HB /=/andP[kA kB].
-      rewrite !is_ko_success// if_same//.
-    - move=> A HA B0 HB0 B HB /=/orP[].
-        by move=>/HA->.
-      by move=>/andP[] _/HB->; rewrite andbF.
+    move=> A HA B0 HB0 B HB/= /= /andP[_].
+    move=>/orP[].
+      by move=>/HA->.
+    by move=>/HB->; rewrite andbF.
   Qed.
 
   Lemma success_has_cut {A}:
     success A -> has_cut A = false.
   Proof.
     elim: A => //.
-    - move=> A HA s B HB/=; case: ifP => dA.
-        rewrite is_dead_is_ko//=; apply: success_is_ko.
-      move=>/success_is_ko->//.
-    - by move=> A HA B0 HB0 B HB/=/andP[]/HA->/HB->; rewrite andbF.
+    move=> A HA B0 HB0 B HB/=/andP[sA sB].
+    rewrite HA// HB// andbF//.
   Qed.
 
-  Lemma has_cut_next_alt {A B b}: 
-    has_cut A -> next_alt b A = Some B -> has_cut B.
+  Lemma failed_has_cut {A}:
+    failed A -> has_cut A = false.
   Proof.
-    elim: A B b => //.
-    - move=>/=[]?//? _ [<-]//.
-    - move=> A HA s1 B HB C b/=.
-      move=>/andP[kA kB].
-      by rewrite !is_ko_next_alt//; rewrite !if_same//.
-    - move=> A HA B0 HB0 B HB C b/=.
-      move=> /orP[].
-        move=> cA.
-        case X: next_alt => // [A'|].
-          case: ifP => //= fA.
-            case Y: next_alt => //[B0'][<-]/=.
-            by rewrite (HA _ _ cA X)//.
-          case: ifP => fB.
-            case Y: next_alt => //[B'|].
-              move=> -[<-]/=; rewrite ?has_cut_clean_success//cA//.
-            case W: next_alt => //[A''].
-            case Z: next_alt => //[B0''][<-]/=.
-            rewrite (HA _ _ cA W)//.
-          move=>[<-]/=; rewrite cA//.
-        case: ifP => //= fA.
-        case: ifP => [sA|sA[<-]]/=; rewrite?cA//.
-        case Y: next_alt => //[B'|].
-          move=>[<-]/=; rewrite cA//.
-        case W: next_alt => //[A'].
-        case Z: next_alt => //[B0'][<-]/=.
-        rewrite (HA _ _ cA W)//.
-      move=>/andP[cB0 cB].
-      case: ifP => /= fA.
-        case X: next_alt => //= [A'].
-        case Y: next_alt => //= [B0'] [<-]/=.
-        rewrite cB0 (HB0 _ _ cB0 Y) orbT//.
-      case: ifP => sA.
-        case X: next_alt => [B'|].
-          move=> [<-]/=; rewrite cB0 (HB _ _ cB X) orbT//.
-        case Y: next_alt => //[A'].
-        case Z: next_alt => //[B0'][<-]/=.
-        by rewrite cB0 (HB0 _ _ cB0 Z) orbT.
-      by move=> [<-]/=; rewrite cB0 cB orbT.
+    elim: A => //.
+    move=> A HA B0 HB0 B HB/=/orP[fA|/andP[sA fB]].
+      rewrite fA//.
+    rewrite success_failed//= success_has_cut//= HB//.
+  Qed.
+
+  Lemma has_cut_next_alt_None {A b}: 
+    next_alt b A = None -> has_cut A = false.
+  Proof.
+    elim: A b => //=.
+    move=> A HA B0 HB0 B HB b.
+    case:ifP => fA//.
+    case:ifP => sA//.
+    case nB: next_alt => [B'|]//=.
+    rewrite (HB b)//=.
+    case nA: next_alt => [A'|]//=; last first.
+      rewrite (HA true)//=.
+    rewrite success_has_cut//.
+  Qed.
+
+  Lemma has_cut_next_alt {A b}: 
+    has_cut A -> next_alt b A = Some A.
+  Proof.
+    elim: A b => //.
+    - move=> A HA B0 HB0 B HB b/= /andP[/eqP fA].
+      rewrite fA.
+      case:ifP => sA//.
+      rewrite success_has_cut//= => cB.
+      rewrite HB//.
   Qed.
 End has_cut.
 
@@ -212,14 +187,24 @@ Section checker.
   Lemma minD_assoc {x y z}: minD x (minD y z) = minD (minD x y) z.
   Proof. case: x => //=; case: y => //=; case: z => //. Qed.
 
-  Definition map_ty {A B} (F: A -> typecheck B) (ob1: typecheck A) : (typecheck B) :=
+  Definition map_ty {A B:eqType} (F: A -> typecheck B) (ob1: typecheck A) : (typecheck B) :=
     match ob1 with
     | ty_err => ty_err
     | ty_ok cnt => F cnt
     end.
 
+  Definition map_ty' {T1 T2:eqType} F t1 :=
+    @map_ty T1 T2 (fun x => ty_ok (F x)) t1.
+
+
   Definition map_ty_bool ob1 ob2 : typecheck bool :=
     map_ty (fun x => map_ty (fun y => ty_ok (x && y)) ob1)  ob2.
+
+  Definition tydflt {T:eqType} dflt (t:typecheck T) :=
+    match t with
+    | ty_ok t => t
+    | ty_err => dflt
+    end.
 
   Fixpoint incl_aux f1 f2 s1 s2 : typecheck _:=
     match s1, s2 with
@@ -270,7 +255,7 @@ Section checker.
     Goal (weak SMap) == WMap. Proof. move=> //=. Qed.
   End test.
 
-  Definition map_ty_opt {A B: Type} (f: A -> typecheck (option B)) t :=
+  Definition map_ty_opt {A B: eqType} (f: A -> typecheck (option B)) t :=
     match t with
     | ty_ok (Some e) => (f e)
     | ty_err => ty_err
@@ -375,7 +360,7 @@ Section checker.
     end.
 
   (* checks inputs and assumes outputs of a callable *)
-  Definition check_callable sP sV (c: Callable) d : typecheck (D * sigV) :=
+  Definition check_callable sP sV (c: Callable) d : typecheck (D * sigV)%type :=
     match check_tm sP sV (Callable2Tm c)  with
     | ty_err => ty_err
     | ty_ok None => ty_ok (Pred, sV)
@@ -388,7 +373,7 @@ Section checker.
       else ty_ok (Pred, sV)
     end.
 
-  Definition check_atom sP sV (a: A) (s:D) : typecheck (D * sigV) :=
+  Definition check_atom sP sV (a: A) (s:D) : typecheck (D * sigV)%type :=
     match a with
     | ACut => ty_ok (Func, sV)
     | ACall t => check_callable sP sV t s
@@ -452,7 +437,7 @@ End checker.
   "((A, A') ; B) , C" is OK if B is dead already (cutr by predecessor of A for example)
 
 *)
-Fixpoint det_tree_aux (sP:sigT) (sV : sigV) A dd : typecheck (D * sigV) :=
+Fixpoint det_tree_aux (sP:sigT) (sV : sigV) A (dd:D) : typecheck (D * sigV)%type :=
   match A with
   | CutS => ty_ok (Func, sV)
   | CallS _ a => 
@@ -470,37 +455,43 @@ Fixpoint det_tree_aux (sP:sigT) (sV : sigV) A dd : typecheck (D * sigV) :=
             ty_ok (maxD ddB0 ddB, sV')) rB) rB0) rA
   | Or A _ B =>
       (* TODO: should use the substitution s before running the check on B?
-         if so, it is no needed to verify that the state is valid
-      *)
+         if so, it is no needed to verify that the state is valid *)
       map_ty (
         fun '(sVA, sV') => 
         map_ty (fun '(sVB, _) =>
-      if has_cut A then ty_ok (maxD sVA sVB, sV) else 
+      if has_cut A || is_ko A then ty_ok (maxD sVA sVB, sV) else 
       if (is_ko B) then ty_ok (sVA, sV')
       else ty_ok (Pred, sV)) (det_tree_aux sP sV B dd)) (det_tree_aux sP sV A dd)
   end.
 
-Definition typ_func (A: typecheck (_ * sigV)) := match A with ty_ok (Func, _) => true | _ => false end.
-
-Definition det_tree sP A := typ_func (det_tree_aux sP empty_ctx A Func).
-
-Lemma no_alt_ko {sP A}: is_ko A -> det_tree sP A.
+Lemma is_ko_det_tree_aux {sP sV A d}:
+  is_ko A -> det_tree_aux sP sV A d = ty_ok(d, sV).
 Proof.
-  rewrite/det_tree.
-  elim: A => //.
-  + move=> A HA s B HB /=/andP[kA kB].
-    case X: det_tree_aux HA => //=[[[] sVA]|]/(_ kA)//.
-    case Y: det_tree_aux HB => //=[[[] sVB]|]/(_ kB)//=.
-    rewrite is_ko_has_cut//.
-  + move=> A HA B0 HB0 B HB /= ->//.
+  elim: A d sV => //=.
+  - move=> A HA s B HB d sV /andP[kA kB].
+    rewrite HA//HB//= kA orbT maxD_refl//.
+  - move=> A HA B0 HB0 B HB d sV ->//.
 Qed.
 
-Lemma no_alt_cut {sP A}: det_tree sP (cutr A).
-Proof. apply: no_alt_ko is_ko_cutr. Qed.
+Lemma is_dead_det_tree_aux {sP sV A d}:
+  is_dead A -> det_tree_aux sP sV A d = ty_ok(d, sV).
+Proof. move=> /is_dead_is_ko /is_ko_det_tree_aux//. Qed.
 
+(* Lemma success_det_tree_aux {sP sV A d}:
+  success A -> det_tree_aux sP sV A d = ty_ok(d, sV).
+Proof.
+  elim: A d sV => //=.
+  - move=> A HA s B HB d sV.
+    case:ifP => [dA sB|dA sA]/=.
+      rewrite HB// is_dead_has_cut//= is_dead_det_tree_aux//=maxD_refl//.
+    rewrite HA//=.
+      rewrite HA//HB//= is_ko_has_cut//=maxD_refl//.
+  - move=> A HA B0 HB0 B HB d sV ->//.
+Qed. *)
 
-Lemma no_alt_dead {sP A}: is_dead A -> det_tree sP A.
-Proof. move=>/is_dead_is_ko. apply: no_alt_ko. Qed.
+Definition typ_func (A: typecheck (_ * sigV)%type) := match A with ty_ok (Func, _) => true | _ => false end.
+
+Definition det_tree sP A := typ_func (det_tree_aux sP empty_ctx A Func).
 
 Lemma all_det_nfa_big_and {sP sV l r} p: 
   typ_func (check_atoms sP sV l r)-> 
@@ -537,195 +528,323 @@ Proof.
   case: det_tree_aux => //-[]//=[]//.
 Qed.
 
-(* Lemma cut_followed_by_det_has_cut {sP sV l} p:
-  check_atoms_w_cut sP sV l -> has_cut (big_and p l).
-Proof. move=>/andP[] _; elim: l => //=-[]//= x xs IH /IH->//. Qed.
-
-Lemma cut_followed_by_det_nfa_and {sP sV bo} p:
-  check_atoms_w_cut sP sV bo -> (det_tree_aux sP sV (big_and p bo) Func).1 = Func.
-Proof. move=>/andP[]/eqP/all_det_nfa_big_and//. Qed. *)
-
 Lemma deterf_empty c: 
   deref empty c = c.
 Proof. elim: c => //= t IH tm H; rewrite IH//. Qed.
 
-(* Lemma tiki_taka {modes sP u q hd s1 c}:
-  tm2RC (Callable2Tm c) = Some q ->
-  H u (modes q) q hd empty = Some s1 ->
-  check_tm sP empty_ctx (Callable2Tm c) = (b (d Func), true)
-   -> rcallable_is_det sP hd.
-Proof.
-  generalize (modes q) => {}modes/=.
-  elim: modes q hd s1 c => //=.
-    move=> []//=k []//= k1 s1 c; case: eqP => //=?+[?]; subst.
-    elim: c k1 => //=.
-      move=> k k1 [<-][->]//.
-    move=> c IH t k1.
-    case: tm2RC => //.
-  move=> [] ms IH []//= r t []//=r1 tm1 s1 []//=r2 tm2.
-    case X: tm2RC => //=[r3][??]; subst.
-    case Y: H => //=[s3] H1.
-    case Z: check_tm => //=[[|m sx sy]b1]//.
-    case: m Z => H2.
-      case W: check_tm => [sw b2].
-      case: ifP => //; case: b1 H2 => //; case: b2 W => //=.
-      move=> H2 W H3 [?]; subst.
-      admit.
-    admit.
-  case X: tm2RC => //=[r3][??]; subst.
-  case Y: H => //=[s3] H1.
-  case Z: check_tm => //=[[|m sx sy]b1]//.
-  case: m Z => H2.
-    case W: check_tm => [sw b2].
-    case: ifP => //; case: b1 H2 => //; case: b2 W => //=.
-    move=> H2 W H3 [?]; subst.
-    admit.
-  admit.
-Admitted. *)
-
-(* Given a deterministic predicate p,
-  Let t, be a valid call to p,
-  Given a list of valid rules in a program p, then
-  backchaining produces a deterministic tree!
-*)
-
-(* Lemma is_det_det_tree {u} {p c sP}:
-  (forall pr : program, check_rules sP empty_ctx (rules pr)) ->
-  (det_tree_aux sP empty_ctx (CallS p c) Func).1 == Func ->
-  (det_tree_aux sP empty_ctx (big_or u p empty c) Func).1 == Func.
-Proof.
-  rewrite/check_rules/=/check_rule.
-  rewrite/=.
-  rewrite /big_or/F.
-  case X: tm2RC => //[rc].
-  move=> /(_ p).
-  case: p => rules modes sig1 /=.
-  generalize {| rules := rules; modes := modes; sig := sig1 |} as pr => pr.
-  clear -X.
-  rewrite/check_callable.
-  elim: rules modes c pr rc X => //=.
-  move=> [] hd bo rules IH modes /= c p q X /andP[Hx Hy].
-  case Y: check_tm => [s []]//=.
-  case: s Y => // -[]//=d H1.
-  case Z: get_callable_hd_sig => //=[s].
-  rewrite maxD_comm/=.
-  case: d H1 => //= H2 _.
-  have {IH} := IH _ _ _ _ X Hy; rewrite H2/=Z/= => -/(_ modes p erefl).
-  case W: run.H => [s1|]//=.
-  move/orP: Hx => [].
-    rewrite deterf_empty in X.
-    admit. (*TODO: hd = q = c and c is func: *)
-  move=>/[dup]/cut_followed_by_det_nfa_and -/(_ p)+H.
-  case R: select => //=[|x xs].
-    case: det_tree_aux => -[]//.
-  case : x R => [sx bx]/=.
-  case T: det_tree_aux => [dy sr]/=+?; subst => /=.
-  case U: det_tree_aux => //=[[] bw]//=+ _.
-  case: ifP => //=.
-  case: ifP => //=.
-  have:= cut_followed_by_det_has_cut _ H.
-  move=> ->//.
-Admitted. *)
-
 (* INVARIANT: all variables are deref  *)
-Fixpoint sigma2ctx (sP:sigT) (s: Sigma) acc : option sigV :=
+Fixpoint sigma2ctx (sP:sigT) (s: Sigma) : seq (typecheck (V * S)%type):=
   match s with
-  | [::] => Some (rev acc)
+  | [::] => [::]
   | (k,v)::xs => 
     match check_tm sP empty_ctx v with
-    | ty_err => None
-    | ty_ok (Some (v, b1)) => sigma2ctx sP xs ((k, if b1 then v else weak v)::acc)
-    | ty_ok None => sigma2ctx sP xs acc
+    | ty_err => [::ty_err]
+    | ty_ok (Some (v, b1)) => (ty_ok (k, if b1 then v else weak v)) :: sigma2ctx sP xs
+    | ty_ok None => sigma2ctx sP xs
     end
   end.
+
+  Definition is_ty_ok {T:eqType} (t:typecheck T) := match t with ty_ok _ => true | _ => false end.
+
+  Lemma check_rules_select {sP sV u l rc m s rules}:
+    check_rules sP sV rules ->
+      select u rc m rules s = l ->
+        check_rules sP sV (map snd l).
+  Proof.
+    move=> +<-{l}.
+    elim: rules => //= -[hd pm]/= rs IH.
+    case cr: check_rule => [[]|]//= /IH {}IH.
+    case X: H => //=[s']; rewrite IH andbT.
+    rewrite cr//.
+  Qed.
+
+Lemma check_callable_pred {sP sV c d s}:
+  check_callable sP sV c Pred = ty_ok (d, s) ->
+    d = Pred.
+Proof.
+  rewrite/check_callable.
+  case: check_tm => //= -[|[]]//.
+  move=> [][]//=[]//D [|[]]//.
+  rewrite maxD_comm/=.
+  case: get_callable_hd_sig; last first.
+    move=> []//.
+  move=> ?; case: assume_call => //=-[[]|??[]]//.
+Qed.
+
+(* Axiom more_precice: sigV -> sigV -> bool. *)
+
+(* Lemma det_tree_aux_func2 {sP sV1 sV2 A d1 d2 f1 f2 sV1' sV2'}:
+  det_tree_aux sP sV1 A d1 = ty_ok (f1, sV1') ->
+    more_precice sV2 sV1 -> 
+    minD d1 d2 = d2 ->
+      minD f1 f2 = f2 ->
+        det_tree_aux sP sV2 A d2 = ty_ok (f2, sV2').
+Proof.
+  elim: A sV s ign => //=; try congruence.
+  - move=> _ c sV s ign.
+    case: ign => //=.
+    case Z: check_callable => //[[]].
+    have ?:= check_callable_pred Z; subst => //.
+  - move=> A HA s B HB sV s1 ign.
+    case: ign => //=.
+    case dtA: (det_tree_aux _ _ A) => // [[dA sVA]]/=.
+    case dtB: (det_tree_aux _ _ B) => // [[dB sVB]]/=.
+    case: ifP => //=cA.
+      destruct dA, dB => //-[?]; subst.
+      rewrite (HA _ _ _ dtA) (HB _ _ _ dtB)//.
+    case: ifP => //= kB.
+    move: dtB => +[??]; subst.
+    rewrite (HA _ _ _ dtA)/= !(is_ko_det_tree_aux kB)//.
+  - move=> A HA B0 HB0 B HB sV sV' ign.
+    case:ifP => kA; try congruence.
+    case: ign => //=.
+    case dtA: (det_tree_aux _ _ A) => // [[dA sVA]]/=.
+    case dtB0: (det_tree_aux _ _ B0) => // [[dB0 sVB0]]/=.
+    case dtB: (det_tree_aux _ _ B) => // [[dB sVB]]/=.
+    move=> [].
+    destruct dB0, dB => // _ ?; subst.
+    case: dA dtA dtB dtB0 => //= dtA dtB dtB0.
+      rewrite (HA _ _ _ dtA)/=dtB dtB0//.
+    have {}HB0 := (HB0 _ _ _ dtB0).
+    have {}HB := (HB _ _ _ dtB).
+    case dtA': (det_tree_aux _ _ A) => // [[[] sVA]|]/=; last first.
+    - admit.
+    - 
+    
+      rewrite HB.
+
+      have:= HA sV _ Pred.
+    case: 
+Qed. *)
+
+Definition same_ty_subst (A B: typecheck (D * sigV)%type) :=
+  (map_ty' snd A) == (map_ty' snd B). 
+
+Lemma check_callable_sama_subst sP sV c D1 D2:
+  same_ty_subst (check_callable sP sV c D1) (check_callable sP sV c D2).
+Proof.
+  rewrite/check_callable/=/same_ty_subst.
+  case X: check_tm => [[[[[|bb]|] []]|]|]//=.
+  case Y: get_callable_hd_sig => [s2|]//=.
+  case Z: assume_call => //=.
+Qed.
+
+Lemma det_tree_aux_same_subst sP sV A d1 d2:
+  same_ty_subst (det_tree_aux sP sV A d1) (det_tree_aux sP sV A d2).
+Proof.
+  rewrite/same_ty_subst.
+  elim: A d1 d2 sV => //=.
+  - move=> _ c d1 d2 sV.
+    have:= check_callable_sama_subst sP sV c d1 d2.
+    do 2 case: check_callable => [[]|]//=.
+  - move=> A HA s B HB d1 d2 sV.
+    have {HA} := HA d1 d2 sV.
+    do 2 case: (det_tree_aux _ _ A) => /=[[??]|]//.
+    have {HB} := HB d1 d2 sV.
+    do 2 case: (det_tree_aux _ _ B) => /=[[??]|]//=.
+    move=> /eqP [?]/eqP[?]; subst.
+    repeat case:ifP => //.
+  - move=> A HA B0 HB0 B HB d1 d2 sV.
+    have {HA} := HA d1 d2 sV.
+    case: (det_tree_aux _ _ A) => /=[[dA sA]|]//;
+    case: (det_tree_aux _ _ A) => /=[[dA' sA']|]//; last first.
+      case:ifP => //.
+    move=>/eqP[->].
+    have {HB0}/= := HB0 dA dA' sA'.
+    do 2 case: (det_tree_aux _ _ B0) => /=[[??]|]//; try by case:ifP.
+    move=> /eqP [?]; subst.
+    have {HB}/= := HB dA dA' sA'.
+    do 2 case: (det_tree_aux _ _ B) => /=[[??]|]//; by case:ifP.
+Qed.
+
+Lemma det_tree_aux_func2 {sP sV A s ign}:
+  det_tree_aux sP sV A ign = ty_ok (Func, s) ->
+    det_tree_aux sP sV A Func = ty_ok (Func, s).
+Proof.
+  elim: A sV s ign => //=; try congruence.
+  - move=> _ c sV s ign.
+    case: ign => //=.
+    case Z: check_callable => //[[]].
+    have ?:= check_callable_pred Z; subst => //.
+  - move=> A HA s B HB sV s1 ign.
+    case: ign => //=.
+    case dtA: (det_tree_aux _ _ A) => // [[dA sVA]]/=.
+    case dtB: (det_tree_aux _ _ B) => // [[dB sVB]]/=.
+    case: ifP => //=cA.
+      destruct dA, dB => //-[?]; subst.
+      rewrite (HA _ _ _ dtA) (HB _ _ _ dtB)//.
+    case: ifP => //= kB.
+    move: dtB => +[??]; subst.
+    rewrite (HA _ _ _ dtA)/= !(is_ko_det_tree_aux kB)//.
+  - move=> A HA B0 HB0 B HB sV sV' ign.
+    case:ifP => kA; try congruence.
+    case: ign => //=.
+    case dtA: (det_tree_aux _ _ A) => //= [[dA sVA]].
+    case dtB0: (det_tree_aux _ _ B0) => //= [[dB0 sVB0]].
+    case dtB: (det_tree_aux _ _ B) => //= [[dB sVB]].
+    move=> [].
+    destruct dB0, dB => // _ ?; subst.
+    case: dA dtA dtB dtB0 => //= dtA dtB dtB0.
+      rewrite (HA _ _ _ dtA)/=dtB dtB0//.
+    have {}HB0 := (HB0 _ _ _ dtB0).
+    have {}HB := (HB _ _ _ dtB).
+    have:= det_tree_aux_same_subst sP sV A Pred Func.
+    rewrite dtA.
+    case dtA': (det_tree_aux _ _ A) => [[dA sVA]|]//={HA}.
+    move=>/eqP[?]; subst.
+    case: dA {dtA'}; rewrite ?HB?HB0//dtB dtB0//.
+Qed.
 
 (* 
   Given a checked program, and a deterministic tree,
   then calling expand produces a tree which is still deterministic.
 *)
-Lemma expand_det_tree {u sP sV sV' A r s} : 
+Lemma expand_det_tree {u sP sVT sV sV' A r s ign} : 
   check_program sP ->
-    sigma2ctx sP s [::] = Some sV ->
-      det_tree_aux sP sV A Func = ty_ok (Func, sV') ->
+    sigma2ctx sP s = sVT ->
+      all is_ty_ok sVT ->
+      map (tydflt (IV 0, b (Exp))) sVT = sV ->
+      det_tree_aux sP sV A ign = ty_ok (Func, sV') ->
         expand u s A = r ->
-          typ_func (det_tree_aux sP sV' (get_tree r) Func).
+          typ_func (det_tree_aux sP sV (get_tree r) Func)
+      
+          (* exists sV'', det_tree_aux sP sV (get_tree r) Func = ty_ok (Func, sV'') *)
+          (*/\ sigma2ctx (get_substS (get_tree r)) \not\incl sV'' *).
 Proof.
-  move=> H ++ <-; clear r.
-  elim: A s sV sV' => //.
-  - move=> p c s sV sV' /=.
+  simpl in *.
+  rewrite/check_program.
+  move=> H; elim: A s sVT sV sV' r ign; try by move => *; subst.
+  - move=> p c s sVT sV sV' r ign /=.
     {
-      rewrite /big_or.
-      case X: F => //=[[sr r]rs]/=.
-      move=> /=.
-      elim: s p c sV sV' => /=.
-      - move=> p c sV sV' []?; subst.
-        rewrite/rev /=.
-        rewrite/check_callable.
-        case X: check_tm => [[[[]d b]|]|]//=.
-        case: d X => //=-[]//=.
-          case: b => //=.
-          case X: get_callable_hd_sig => //[s].
-          case Y: assume_call => //=[sV''] + [?]; subst.
-          rewrite/big_or.
-        
-
-        Search "rev" "nil".
+      rewrite /big_or/F.
+      have /= := H p.
+      case: p => rules modes sig1 /=.
+      generalize {| rules := rules; modes := modes; sig := sig1 |} as pr => pr.
       clear -H.
+      case: ign => //=; last first.
+        case X: check_callable => //[[dA sVA]].
+        have ? := check_callable_pred X; subst => //.
+      rewrite/check_callable.
+      case cc: check_tm => //=[[[[[|d]|] []]|]]//=.
+      case sign: get_callable_hd_sig => //[sig_of_c].
+      case assm: assume_call => //=[sc'].
+      case: d cc => //= +++++ [?]; subst.
+      case tmC: tm2RC => [rc|]; try by move=> *; subst.
+      case mode: lookup => [m|]; try by move=> *; subst.
+      case sel: select => [|[sx x] xs]/=; try by move=> *; subst.
+      move=> good_call H2 ? H3 ??; subst => /=.
+      have /= := check_rules_select H2 sel.
+      case cpx: check_rule => [[]|]//= cxs.
+      clear sel.
+      remember (map (tydflt (IV 0, b Exp)) (sigma2ctx sP s)) as sV eqn:HsV.
+      simpl in sV.
+      case: x cpx => /= hd0 pm0 cr0.
+      clear rules H2.
+      clear m mode rc tmC modes.
+      rewrite-HsV.
+      admit.
     }
-    move: H.
-    rewrite /check_program.
-    apply is_det_det_tree.
-  - move=> A HA s B HB/=.
-    case X: det_tree_aux => [dA sA].
-    case Y: det_tree_aux => [dB sB].
-    case: ifP => /=.
-      case: dA X => //=; case: dB Y => //= H1 H2 H3 _.
-      case: ifP => DA.
-        rewrite get_tree_Or/= H2/=.
-        move: HB; rewrite H1/=H3 => /(_ erefl).
-        (* TODO: the IH for is not enough generalized... *)
-        admit.
-      move: HA; rewrite H2/= => -/(_ erefl).
-      have:= @expand_has_cut u _ empty H3.
-      case X: expand => //=[s' A'|s' A'|A'|s' A']; 
-      case d: det_tree_aux => //=[s2 sA']; try by move=> []//->/eqP->; rewrite H1//.
-      rewrite is_ko_cutr=> + /eqP?; subst =>/=.
-      have:= @no_alt_cut sP B; rewrite /det_tree.
-      case: det_tree_aux => //= -[]// _ _; case:ifP => //.
-    case: ifP => //; case: dA X => //= X kB cA _.
-    rewrite (is_ko_expand _ kB)/=.
-    case: ifP => dA/=.
-      rewrite X Y cA kB//.
-    move: HA; rewrite X => -/(_ erefl).
-    case e: expand => //=[s' A'|s' A'|A'|s' A']/eqP; try by
-      case: det_tree_aux => -[]//= b _; rewrite Y kB;
-      have:= @no_alt_ko sP B kB;
-      rewrite/det_tree Y => /eqP/=->; case: ifP => //.
-    case: det_tree_aux => -[]//=.
-    have:= @no_alt_cut sP B.
-    rewrite/det_tree.
-    case: det_tree_aux => -[]//= _ _ b _; rewrite is_ko_cutr; case: ifP => //.
-  - move=> A HA B0 HB0 B HB /=.
-    case: ifP => kA.
-      rewrite (is_ko_expand _ kA)/=kA//.
-    move: HA; case dA: det_tree_aux => //=[DA SA] {}HA.
-    (* case: ifP. *)
-    (* move=> /eqP->. *)
-    case dB0: det_tree_aux => //[DB0 SB0]/=.
-    case dB: det_tree_aux => //[DB SB]/=.
-    case: DB0 dB0 => //=; case: DB dB => //= DB DB0 _.
-    move: HA; case e: expand => //=[s' A'|s' A'|A'|s' A']; 
-    rewrite ?eqxx; try case: ifP => //=.
-      case dt: det_tree_aux => //=[dx sx].
-      case: DA dA DB DB0 => //=.
-        move=> ++++/(_ erefl)/eqP?; subst.
+  - move=> A HA s B HB/=s1 sVT sV sV' r ign.
+    case: (ifP (is_dead A)) => DA.
+      {
+        move=> ++++<-; rewrite get_tree_Or/=.
+        rewrite !(is_dead_det_tree_aux DA)//=.
+        rewrite is_dead_is_ko// orbT//=.
+        case dtB : det_tree_aux => //=[[[] sB]]//=; rewrite (@maxD_comm ign)//=.
+        case: ign dtB => //dtB.
+        move=> +++[?]; subst => H1 H2 H3.
+        have {HA HB} := HB _ _ _ _ _ _ H1 H2 H3 dtB erefl.
+        (* TODO: s is in the Or, it should be a more precise instance of s, by hyp on a valid state *)
+        have? : s = s1 by admit.
+        subst s1.
+        by case X: det_tree_aux => //=[[[] sVB']]//= _.
+      }
+      move=> ++++<-.
+      case dtA: (det_tree_aux _ _ A) => //=[[dA sVA]].
+      case dtB: (det_tree_aux _ _ B) => //=[[dB sVB]].
+      case: ifP => //.
+        destruct dA, dB => //= ++++[?]; subst.
+        move=> /orP[]; last first.
+          move=> kA.
+          rewrite is_ko_expand//= kA orbT.
+          rewrite (is_ko_det_tree_aux kA)//=.
+          move=> // H1 H2 H3.
+          by rewrite (det_tree_aux_func2 dtB)//.
+        move=> cA H1 H2 H3.
+        have {HA} := HA _ _ _ _ _ _ H1 H2 H3 dtA erefl.
+        (* TODO: s is in the Or, it should be a more precise instance of s, by hyp on a valid state *)
+        have? : s = s1 by admit.
+        subst s1.
+        case eA: expand => [A'|A'|A'|A']; rewrite?orbT?orbF/=.
+        - case: det_tree_aux => //= -[] []//= ? _ ; rewrite (det_tree_aux_func2 dtB)//=.
+          have cA' : has_cut A' by admit.
+          rewrite cA'//.
+        - rewrite is_ko_cutr (is_ko_det_tree_aux is_ko_cutr)/=.
+          case: det_tree_aux => //-[]/=[]//=*; case: ifP => //.
+        - rewrite (det_tree_aux_func2 dtB)/=; case: det_tree_aux => //=-[][]//=.
+          have cA' : has_cut A' by admit.
+          rewrite cA'//.
+        - rewrite (det_tree_aux_func2 dtB)/=; case: det_tree_aux => //=-[][]//=.
+          have cA' : has_cut A' by admit.
+          rewrite cA'//.
+      case cA:has_cut => //=kA.
+      case: ifP => //kB.
+      move: dtB; rewrite is_ko_det_tree_aux//= => -[??]; subst.
+      move=> H1 H2 H3 [??]; subst dA sVA.
+      have {HA} := HA _ _ _ _ _ _ H1 H2 H3 dtA erefl.
+      case eA: expand => [A'|A'|A'|A']; rewrite?orbT?orbF/=. 
+      - case: det_tree_aux => //-[][]//= sV'' _.
+        by rewrite is_ko_det_tree_aux//= kB; case:ifP.
+      - rewrite is_ko_cutr.
+        case: det_tree_aux => //-[][]//= sV'' _.
+        rewrite is_ko_det_tree_aux//=?is_ko_cutr//;case:ifP => //.
+      - case: det_tree_aux => //-[][]//= sV'' _.
+        by rewrite is_ko_det_tree_aux//= kB; case:ifP.
+      - case: det_tree_aux => //-[][]//= sV'' _.
+        by rewrite is_ko_det_tree_aux//= kB; case:ifP.
+  - move=> A HA B0 _ B HB s sVT sV sV' r/= ign.
+    case:ifP => kA/=.
+      rewrite is_ko_expand//=.
+      move=> H1 H2 H3 [??]<-/=; rewrite kA//.
+    case dtA: (det_tree_aux _ _ A) => //=[[dA sVA]].
+    case dtB0: (det_tree_aux _ _ B0) => /=[[dB0 sVB0]|]//=.
+    case dtB: (det_tree_aux _ _ B) => /=[[dB sVB]|]//=.
+    move=> H1 H2 H3; destruct dB0, dB => //-[?] <-; subst sV'.
+    case X: expand => //=[A'|A'|A'|A']; try case: ifP => //kA'.
+    - case Y: det_tree_aux => //=[[DA sVA']|]; last first.
+         admit. (*not possyble: expand always return a typecheckable tree*)
+      have ? : sVA = sVA' by admit.
+      subst sVA'.
+      have ? : DA = dA by admit.
+      subst DA. 
+      rewrite dtB dtB0//.
+    - case Y: det_tree_aux => //=[[DA sVA']|]; last first.
+        admit. (*not possyble: expand always return a typecheckable tree*)
+      have ? : sVA = sVA' by admit.
+      subst sVA'.
+      have ? : DA = dA by admit.
+      subst DA; rewrite dtB dtB0//.
+    - have [? fA]:= expand_failed_same _ X.
+      have ? : sVA = sV by admit.
+      subst sVA A'.
+      have:= det_tree_aux_same_subst sP sV A ign Func.
+      rewrite dtA.
+      case W: det_tree_aux => /=[[DA' sVA'']|]//.
+      move=> /eqP [?]; subst sVA''.
+      case: DA' W => //=.
+        rewrite (det_tree_aux_func2 dtB)(det_tree_aux_func2 dtB0)//.
+      admit.
+    - have [? fA]:= expand_solved_same _ X.
+      have ? : sVA = sV by admit.
+      subst sVA A'.
+      case eB : expand => [B'|B'|B'|B']/=; rewrite ?is_ko_cutl?success_is_ko//=.
 Admitted.
 
-Lemma expand_det_tree {u sP A r} : 
+(* Lemma expand_det_tree {u sP A r} : 
   check_program sP -> det_tree sP A -> 
     expand u empty A = r ->
       det_tree sP (get_tree r).
-Proof.
+Proof. *)
 
 (* Lemma expand_next_alt {u sP s1 A s2 B} : 
   check_program sP -> det_tree sP A ->
@@ -750,7 +869,8 @@ Proof.
   - move=> A HA B0 _ B HB s1 C s2 /=.
     move=>/orP[].
       move=> kA; rewrite is_ko_expand//.
-    move=> /and3P[/orP[/andP[cB0 cB]|fA] fB fB0].
+    move=> /and3P-- 
+Davide Fissore[/orP[/andP[cB0 cB]|fA] fB fB0].
       case X: expand => // [s3 D].
       have:= HB s3 _ _ fB.
       have sbF:= has_cut_success cB.
@@ -763,209 +883,357 @@ Proof.
     by rewrite H1 H2; rewrite !if_same.
 Qed. *)
 
-Lemma det_tree_next_alt {sP s1 A s2 B}:
-  det_tree sP A -> next_alt s1 A = Some (s2, B) -> det_tree sP B.
+Lemma det_tree_next_alt {sP sV A B any}:
+  det_tree_aux sP sV A any = ty_ok (Func, sV) ->
+    next_alt false A = Some B -> 
+      det_tree_aux sP sV B Func = ty_ok (Func, sV).
 Proof.
-  elim: A s1 B s2 => //.
-  - move=> []//??? _ [_<-]//.
-  - move=>/=??[]//??? _ [_<-]//.
-  - move=> []//??? _ [_<-]//.
-  - move=> A HA s B HB s1 C s2 /=.
-    move=>/andP[fA].
-    case: (ifP (is_dead _)) => dA.
-      rewrite is_dead_has_cut//.
-      move=> fB.
-      have:= HB (Some s) _ _ fB.
-      case X: next_alt => //[[s3 D]] /(_ _ _ erefl) fD[_ <-]/=.
-      rewrite no_alt_dead// is_dead_has_cut// fD.
-    case: ifP => cA.
-      move=> fB.
-      have:= (HA s1 _ _ fA).
-      case X: next_alt => //[[s3 D]|].
-        have cD:= has_cut_next_alt cA X.
-        by move=> /(_ _ _ erefl) fD[_<-]/=; rewrite fD cD fB.
-      move=> _.
-      case: ifP => dB//.
-      have idA := @is_dead_dead A.
-        case Y: next_alt => //[[s3 D]].
-        move=>[_ <-]/=.
-        rewrite no_alt_dead// is_dead_has_cut//.
-        apply: HB fB Y.
-    move=>/eqP->; rewrite (is_ko_next_alt is_ko_cutr) if_same.
-    have:= HA s1 _ _ fA.
-    case: next_alt => // [[s3 D]]/(_ _ _ erefl) fD [_ <-]/=.
-    by rewrite fD cutr2 eqxx no_alt_cut if_same.
-  - move=> A HA B0 HB0 B HB s1 C s2 /=.
-    case: (ifP (is_dead _)) => dA//.
-    move=>/orP[].
-      move=>kA.
-      by rewrite is_ko_failed// is_ko_next_alt//.
-    move=> /and3P[/orP[/andP[cB0 cB]|fA] fB fB0].
-      case: ifP => // fA.
-        case: next_alt => // [[s3 D]]; case: ifP => // _ [_ <-]/=.
-        by rewrite cB0 fB0 orbT.
-      have:= HB s1 _ _ fB.
-      case X: next_alt => // [[s3 D]|].
-        by move=> /(_ _ _ erefl) fD [_ <-]/=; rewrite cB0 (has_cut_next_alt cB X) fD fB0 orbT.
-      move=> _; case: next_alt => // [[s3 D]]; case: ifP => // _ [_ <-]/=.
-      by rewrite cB0 fB0 orbT.
-    case: ifP => // _.
-      have:= HA s1 _ _ fA.
-      case X: next_alt => // [[s3 D]].
-      move=> /(_ _ _ erefl) fD; case: ifP => // _ [_ <-]/=.
-      by rewrite fD orbT fB0 orbT.
-    have:= HB s1 _ _ fB.
-    case: next_alt => // [[s3 D]|].
-      by move=> /(_ _ _ erefl) fD [_ <-]/=; rewrite fA fD fB0 !orbT.
-    move=> _.
-    have:= HA s1 _ _ fA.
-    case X: next_alt => // [[s3 D]].
-    move=> /(_ _ _ erefl) fD; case: ifP => // _ [_ <-]/=.
-    by rewrite fD orbT fB0 orbT.
+  elim: A B sV any => //=.
+  - move=> ??? [<-]//[<-]//.
+  Admitted.
+
+Definition is_det A := forall u s s' B n,
+  runb u s A s' B n -> is_dead B.
+
+Lemma success_det_tree_next_alt {sP A sV1 sV2 ign}:
+  success A -> (det_tree_aux sP sV1 A ign) = ty_ok (Func, sV2) ->
+    (ign = Func /\ is_dead (build_na A (next_alt true A)))%type2.
+Proof.
+  simpl in sV2.
+  elim: A sV1 sV2 ign => //=.
+  - move=> sV1 sV2 ign _ [<-]//.
+  - move=> A HA s B HB sV1 sV2 ign.
+    case:ifP => [dA sB|dA sA].
+      rewrite is_dead_is_ko//orbT is_dead_next_alt//=.
+      rewrite (is_dead_det_tree_aux dA)//=.
+      case X: det_tree_aux => //=[[dB sVB]][??]; subst.
+      destruct ign, dB => //=.
+      have:= (HB _ _ _ sB X).
+      case nB: next_alt => [B'|]/=; rewrite?is_dead_dead//=.
+      move=> [_->]; rewrite dA//.
+    rewrite success_has_cut//=.
+    case dtA: (det_tree_aux _ _ A) => //=[[DA sVA]].
+    case dtB: (det_tree_aux _ _ B) => //=[[DB sVB]].
+    rewrite success_is_ko//=.
+    case:ifP => kB[??]//; subst.
+    have [-> +] := HA _ _ _ sA dtA.
+    case nA: next_alt => [A'|]/=.
+      rewrite (next_alt_dead nA)//.
+    rewrite is_ko_next_alt//=!is_dead_dead//.
+  - move=> A HA B0 HB0 B HB sV1 sV2 ign /andP[sA sB].
+    rewrite success_is_ko//=sA success_failed//=.
+    case dA: (det_tree_aux _ _ A) => //=[[DA sVA]].
+    case dB0: (det_tree_aux _ _ B0) => //=[[DB0 sVB0]].
+    case dB: (det_tree_aux _ _ B) => //=[[DB sVB]].
+    move=>[??]; subst.
+    destruct DB0, DB => //=.
+    have [?]:= HB _ _ _ sB dB; subst.
+    have [?]:= HA _ _ _ sA dA; subst.
+    case nB: next_alt => [B'|]/=.
+      rewrite (next_alt_dead nB)//.
+    case nA: next_alt => [A'|]/=.
+      rewrite (next_alt_dead nA)//.
+    rewrite is_dead_dead//.
 Qed.
 
-(* Lemma expand_next_alt_failed {sP A B C s s'}:
-  check_program sP ->
-    det_tree sP A -> expand u s A = Failure B ->
-      forall sN, next_alt sN B = Some (s', C) -> det_tree sP C.
+Lemma failed_det_tree_next_alt {sP A B sV1 sV2}:
+  failed A ->
+  det_tree_aux sP sV1 A Func = ty_ok (Func, sV2) ->
+    next_alt false A = Some B ->
+      (typ_func (det_tree_aux sP sV1 B Func))%type2.
 Proof.
-  move=> Hz.
-  elim: A B C s s' => //.
-  - move=> /=????? []<-//.
-  - move=> /=????? []<-//.
-  - move=> A HA s1 B HB C D s s' /=++sN.
-    move=>/andP[fA].
-    case: (ifP (is_dead _)) => dA.
-      rewrite is_dead_has_cut// => fB.
-      have:= HB _ _ s1 _ fB.
-      case: expand => // E /(_ _ _ _ erefl (Some s1)) + [<-]/=.
-      rewrite dA.
-      case: next_alt => //[[s2 F]] /(_ _ _ erefl) + [_<-]/=.
-      by move=> /= ->; rewrite is_dead_has_cut// no_alt_dead.
-    case: ifP => //.
-      have := HA _ _ s _ fA _ sN.
-      case X: expand => // [E] /(_ _ _ _ erefl) + cA + [?]; subst.
-      rewrite /= (expand_not_dead _ dA X).
-      have:= @expand_has_cut _ s cA; rewrite X/= => -[]// cE.
-      case Y: next_alt => //[[s2 F]|].
-        move=> /(_ _ _ erefl) fF fB [_ <-] /=.
-        have cF:= has_cut_next_alt cE Y.
-        by rewrite fF cF fB.
-      move=>_ fB.
-      case: ifP => // dB.
-      have dDe := @is_dead_dead E.
-        case nB : next_alt => //= [[s2 F]] [_<-]/=.
-        rewrite no_alt_dead// is_dead_has_cut// (det_tree_next_alt fB nB)//.
-    move=> cA /eqP->.
-    have:= HA _ _ s _ fA _ sN.
-    case X: expand => // [E] /(_ _ _ _ erefl) + [<-]/=.
-    have kcB := @is_ko_cutr B.
-    rewrite /= (expand_not_dead _ dA X) (is_ko_next_alt kcB).
-    rewrite if_same.
-    case Y: next_alt => //[[s2 F]].
-    move=> /(_ _ _ erefl) fF [_ <-] /=.
-    by rewrite fF no_alt_cut cutr2 eqxx if_same.
-  - move=> A HA B0 _ B HB C D s s' /= ++sN.
-    move=> /orP[].
-      move=> kA; rewrite is_ko_expand// => -[<-]/=.
-      rewrite is_ko_failed// is_ko_next_alt// if_same//.
-    move=> /and3P[/orP[/andP[cB0 cB]|fA] fB fB0].
-      case X: expand => //[E|s1 E].
-        move=> [<-]/=.
-        case: ifP => // dS.
-        case: ifP => // fS.
-          case nE: next_alt => [[s3 F]|]//.
-          by case: ifP => //FB0 [_<-]/=; rewrite cB0 fB0 orbT.
-        case Y: next_alt => //[[s3 F]|].
-          by move=>[_ <-]/=; rewrite cB0 (has_cut_next_alt cB Y) fB0 (det_tree_next_alt fB Y) orbT.
-        by case: next_alt => // [[s3 F]]; case:ifP=>//_[_<-]/=; rewrite cB0 fB0 orbT.
-      have:= HB _ _ s1 _ fB _ sN.
-      case Z: expand => // [F] /(_ _ _ _ erefl) + [<-]/=.
-      case: ifP => //dE; case:ifP=>FE.
-        move=> _.
-        by case: next_alt => //[[s3 G]]; case:ifP=>//_[_<-]/=; rewrite cB0 fB0 orbT.
-      case Y: next_alt => //[[s3 G]|].
-        move=>/(_ _ _ erefl) nG.
-        have := @expand_has_cut _ s1 cB.
-        rewrite Z/==>-[]//cF.
-        by move=>[_ <-]/=; rewrite cB0 nG fB0 (has_cut_next_alt cF Y) orbT.
-      have [??]:= expand_solved_same _ X; subst => _.
-      case W: next_alt => //[[s3 G]]; case: ifP => // _[_<-]/=.
-      by rewrite cB0 fB0 orbT.
-    have:= HA _ _ s _ fA _ sN.
-    case X: expand => //[E|s1 E].
-      move=> /(_ _ _ _ erefl) + [<-]/=.
-      case: ifP => // dS.
-      case: ifP => //fE.
-        case: next_alt => //[[s4 G]] /(_ _ _ erefl) fG.
-        by case: ifP => // _[_<-]/=; rewrite fB0 fG orbT orbT.
-      case Y: (next_alt sN B) => //[[s4 G]|].
-        by move=> _ [_<-]/=; rewrite (det_tree_next_alt fB Y) fB0 (expand_det_tree Hz fA X) orbT orbT.
-      case: next_alt => //[[s3 G]] /(_ _ _ erefl)fG; case:ifP=>//_[_<-]/=.
-      by rewrite fG fB0 orbT orbT.
-    move=> _.
-    have:= HB _ _ s1 _ fB _ sN.
-    case Z: expand => // [F] /(_ _ _ _ erefl) {}HB [<-]/=.
-    have /= fE := expand_det_tree Hz fA X.
-    case: ifP => //dE; case:ifP=>FE.
-      case W: next_alt => //[[s3 G]]; case:ifP=>//_[_<-]/=.
-      by rewrite fB0 (det_tree_next_alt fE W) orbT orbT.
-    move: HB.
-    case W: next_alt => //[[s3 G]|].
-      move=> /(_ _ _ erefl) fG [_<-]/=; rewrite fG fB0 fE orbT orbT//.
-    case T: next_alt => //[[s3 G]] => _; case:ifP => //[fB01][_<-]/=.
-    by rewrite fB0 (det_tree_next_alt fE T) orbT orbT.
-  Qed. *)
+  (* elim: A B sV1 sV2 => //=.
+  - move=> A HA s B HB C sV1 sV2.
+    case:ifP => [dA fB|dA fA].
+      rewrite is_dead_is_ko//= is_dead_next_alt//=orbT.
+      rewrite (is_dead_det_tree_aux dA)//=.
+      case dtB: det_tree_aux => //=[[dB sVB]]/=[+?]; subst.
+      destruct dB => //= _.
+      case nB: next_alt => //=[B'][<-]/=.
+      rewrite is_dead_is_ko// (is_dead_det_tree_aux dA)//= orbT.
+      have:= HB _ _ _ fB dtB nB.
+      case dtB': det_tree_aux => //=[[[] sVB']]//=.
+    case dtA: (det_tree_aux _ _ A) => /=[[DA sVA]|]//=.
+    case dtB: (det_tree_aux _ _ B) => /=[[DB sVB]|]//=.
+    case: ifP.
+      move=> +[??]; subst.
+      destruct DA, DB => //.
+      move=> /orP[]; last first.
+        move=> kA; rewrite is_ko_next_alt//=.
+        case nB: next_alt => [B'|]//=[<-]{C}/=.
+        rewrite is_dead_is_ko?is_dead_dead//=orbT/=.
+        rewrite (is_dead_det_tree_aux is_dead_dead)/=.
+        move: dtA; rewrite is_ko_det_tree_aux//= =>-[?]; subst => /=.
+        case fB: (failed B).
+          have := HB _ _ _ fB dtB nB.
+          by case X: det_tree_aux => //[[[] svB]]//=.
+        move: nB; rewrite next_alt_not_failed// => -[?]; subst.
+        rewrite dtB//.
+      move=> cA.
+      case nA: next_alt => [A'|]//=.
+        move=>[<-]{C}.
+        have {HA} := HA _ _ _ fA dtA nA.
+        case dtA': det_tree_aux => /=[[[] sVA']|]//=; repeat split.
+        have /= := next_alt_failed nA.
+        move=> /failed_is_ko->; rewrite orbF.
+        rewrite (has_cut_next_alt cA nA) dtA'//=.
+        rewrite dtB//=.
+      case nB: next_alt => [B'|]//=[<-]{C}/=.
+      rewrite is_dead_is_ko?is_dead_dead//orbT (is_dead_det_tree_aux is_dead_dead)/=.
+      case fB: (failed B).
+        have := HB _ _ _ fB dtB nB; subst.
+        by case X: det_tree_aux => //[[[] svB]]//=.
+      move: nB; rewrite next_alt_not_failed// => -[?]; subst => /=.
+      rewrite dtB//=; rewrite maxD_comm/=.
+    case cA: has_cut => //= kA.
+    case: ifP => kB [??]//; subst.
+    move: dtB; rewrite is_ko_det_tree_aux//(is_ko_next_alt _ kB)//=.
+    move=> [??]; subst.
+    case nA: next_alt => //[A'][<-]{C}/=.
+    have {HA} := HA _ _ _ fA dtA nA.
+    have:= next_alt_failed nA => /failed_is_ko ->; rewrite orbF.
+    case dA': det_tree_aux => /=[[[] sVA']|]//= _.
+    rewrite kB is_ko_det_tree_aux//=; case:ifP => //.
+  - move=> A HA B0 HB0 B HB C sV1 sV2 /orP[fA|/andP[sA fB]].
+      rewrite fA.
+      case: ifP => kA.
+        by rewrite is_ko_next_alt//=.
+      case dtA: det_tree_aux => /=[[DA sVA]|]//=.
+      case dtB0: (det_tree_aux _ _ B0) => /=[[DB0 sVB0]|]//=.
+      case dtB: (det_tree_aux _ _ B) => /=[[DB sVB]|]//=.
+      destruct DB0, DB => //=-[?]; subst.
+      case nA: next_alt => //=[A'].
+      case nB0: next_alt => //=[B0'][<-]{C}/=.
+      have:= next_alt_failed nA => /failed_is_ko ->. *)
+Abort.
 
-(* Lemma expandedb_next_alt_failed {sP s A B C s' b1}: 
-  check_program sP ->
-    det_tree sP A ->
-      expandedb u s A (Failed B) b1 -> 
-        forall sN, next_alt sN B = Some (s', C) -> det_tree sP C.
+(* Lemma has_cut_next_alt_same {A B b}: 
+  has_cut A = false -> next_alt b A = Some B -> has_cut B = false.
 Proof.
-  remember (Failed _) as f eqn:Hf => Hz + H.
-  elim: H B C s' Hf => //; clear -Hz.
-  - move=> s A B HA ? C s' [<-] fA nB.
-    apply: expand_next_alt_failed Hz fA HA nB.
-  - move=> s s' r A B b HA HB IH C D s1 ? fA sN nB; subst.
-    apply: IH erefl (expand_det_tree Hz fA HA) _ nB.
-  - move=> s s' r A B b HA HB IH C D s1 ? fA sN nB; subst.
-    apply: IH erefl (expand_det_tree Hz fA HA) _ nB.
+  elim: A B b => //=.
+  - move=> B []// _ [<-]//.
+  - move=> p c B// _ _ [<-]//.
+  - move=> A HA s B HB C b _.
+    case nA: next_alt => [A'|]//=.
+      move=> [<-]{C}//.
+    case nB: next_alt => [B'|]//=[<-]{C}//.
+  - move=> A HA B0 HB0 B HB C b.
+    case fA: (failed A) => //=.
+      case nA: next_alt => [A'|]//=.
+      case nB0: next_alt => [B0'|]//= _ [<-]{C}/=.
+
+      ca
+    case: eqP => //=fA.
+      rewrite fA.
+    /andP[/eqP fA]. ; rewrite fA => /orP[cA|cB].
+      rewrite has_cut_success//==>-[<-]{C}/=; rewrite cA fA//.
+    rewrite (has_cut_next_alt cB) if_same => -[<-]{C}/=.
+    rewrite fA cB orbT//.
 Qed. *)
 
-Definition is_det A := forall s s' B,
-  run u s A s' B -> forall s2, next_alt s2 B = None.
+(* 
+Lemma failed_det_tree_next_alt {sP A B sV1 sV2 ign}:
+  (* failed A -> *)
+  det_tree_aux sP sV1 A ign = ty_ok (Func, sV2) ->
+    next_alt false A = Some B ->
+      (typ_func (det_tree_aux sP sV1 B ign))%type2.
+Proof.
+  elim: A B sV1 sV2 ign => //=.
+  - move=> ???? [->->][<-]//.
+  - move=> p c B sv1 sv2 ign + [<-]{B}/=.
+    case ck: check_callable => //=[[DA sVA]] [+ _ {sv2}].
+    destruct DA, ign => //=.
+  - move=> B sv1 sv2 ign [->][<-]//=.
+  - move=> A HA s B HB C sV1 sV2 ign.
+    rewrite if_same.
+    case kA:is_ko => //; rewrite ?orbT ?orbF.
+      rewrite is_ko_next_alt// (is_ko_det_tree_aux kA)/=.
+      case dtB: det_tree_aux => //=[[dB sVB]]/=[+?]; subst.
+      destruct ign, dB => //= _.
+      case nB: next_alt => //=[B'][<-]/=.
+      have /= fB' := next_alt_failed nB.
+      rewrite (failed_is_ko fB')//=.
+      rewrite (fun_if has_cut) (fun_if is_ko) (fun_if (fun x => det_tree_aux sP sV2 x Func)).
+      rewrite (is_ko_det_tree_aux kA).
+      rewrite (is_dead_det_tree_aux is_dead_dead) if_same/=.
+      rewrite failed_has_cut?is_ko_failed//.
+      rewrite failed_has_cut?is_dead_failed?is_dead_dead//=if_same/=.
+      rewrite kA is_dead_is_ko?is_dead_dead//= if_same.
+      have:= HB _ _ _ _ dtB nB.
+      case dtB': det_tree_aux => //=[[[] sVB']]//=.
+    case:ifP => dA.
+      rewrite is_dead_next_alt// (is_dead_det_tree_aux dA)/=.
+      rewrite failed_has_cut?is_dead_failed//=.
+      case:ifP => kB.
+        by rewrite is_ko_det_tree_aux//= is_ko_next_alt//.
+      by case dtB: det_tree_aux => //=[[dB sVB]]/=; subst => //.
+    case dtA: (det_tree_aux _ _ A) => /=[[DA sVA]|]//=.
+    case dtB: (det_tree_aux _ _ B) => /=[[DB sVB]|]//=.
+    case: ifP => cA.
+      move=> [??]; subst.
+      destruct DA, DB => //.
+      rewrite has_cut_next_alt//= => -[<-]{C}/=.
+      rewrite cA/= dtA/=dtB//.
+    case:ifP => //kB[??]; subst.
+    rewrite (is_ko_next_alt _ kB)/=.
+    case nA: next_alt => //=[A'][<-]{C}/=.
+    have /= fA':= next_alt_failed nA.
+    rewrite (failed_is_ko)//=orbF kB.
+    have {HA}:= HA _ _ _ _ dtA nA.
+    case dtA' : det_tree_aux => //=[[[] sVA']]//= _.
+    move: dtB; rewrite is_ko_det_tree_aux//=.
+    move=> [??]; subst DB sVB.
+    case:ifP => //= cA'. *)
 
-Lemma runb_next_alt {sP A}: 
+Lemma failed_det_tree_next_alt {sP A B sV1 sV2 ign}:
+  failed A ->
+  det_tree_aux sP sV1 A ign = ty_ok (Func, sV2) ->
+    next_alt false A = Some B ->
+      (ign = Func /\ typ_func (det_tree_aux sP sV1 B ign))%type2.
+Proof.
+  elim: A B sV1 sV2 ign => //=.
+  - move=> A HA s B HB C sV1 sV2 ign.
+    case:ifP => [dA fB|dA fA].
+      rewrite is_dead_is_ko//= is_dead_next_alt//=orbT.
+      rewrite (is_dead_det_tree_aux dA)//=.
+      case dtB: det_tree_aux => //=[[dB sVB]]/=[+?]; subst.
+      destruct ign, dB => //= _.
+      case nB: next_alt => //=[B'][<-]/=.
+      rewrite is_dead_is_ko// (is_dead_det_tree_aux dA)//= orbT.
+      have:= HB _ _ _ _ fB dtB nB.
+      case dtB': det_tree_aux => //=[[[] sVB']]//=.
+    rewrite failed_has_cut//=.
+    case dtA: (det_tree_aux _ _ A) => /=[[DA sVA]|]//=.
+    case dtB: (det_tree_aux _ _ B) => /=[[DB sVB]|]//=.
+    case: ifP => kA.
+      move=> [??]; subst.
+      destruct DA, DB => //.
+      rewrite is_ko_next_alt//=.
+      case nB: next_alt => //=[B'][<-]{C}/=.
+      rewrite (is_dead_is_ko is_dead_dead) orbT.
+      rewrite (is_dead_det_tree_aux (is_dead_dead))/=.
+      move: dtA; rewrite is_ko_det_tree_aux // => -[??]; subst.
+      case fB: (failed B) => //=.
+        have [_]:= (HB _ _ _ _ fB dtB nB).
+        by case X: det_tree_aux => [[[]]|]//=.
+      move: nB; rewrite next_alt_not_failed// => -[<-]{B'}.
+      by rewrite dtB//.
+    case:ifP => //kB[??]; subst.
+    rewrite (is_ko_next_alt _ kB)/=.
+    case nA: next_alt => //=[A'][<-]{C}/=.
+    have /= fA':= next_alt_failed nA.
+    rewrite (failed_is_ko)//= kB.
+    have [?] := HA _ _ _ _ fA dtA nA; subst.
+    case dtA' : det_tree_aux => //=[[[] sVA']]//= _.
+    rewrite dtB//=.
+    move: dtB; rewrite is_ko_det_tree_aux//= => -[??]; subst.
+    case:ifP => //.
+  - move=> A HA B0 HB0 B HB C sV1 sV2 ign.
+    move=> /orP[fA|/andP[sA fB]].
+      rewrite fA; case:ifP => kA.
+        rewrite is_ko_next_alt//.
+      case dtA: (det_tree_aux _ _ A) => /=[[DA sVA]|]//=.
+      case dtB0: (det_tree_aux _ _ B0) => /=[[DB0 sVB0]|]//=.
+      case dtB: (det_tree_aux _ _ B) => /=[[DB sVB]|]//=.
+      move=>[??]; subst.
+      destruct DB0, DB => //.
+      case nA: next_alt => [A'|]//=.
+      case nB0: next_alt => [B0'|]//=.
+      move=>[<-]{C}/=.
+      have /= fA':= next_alt_failed nA.
+      rewrite (failed_is_ko)//=.
+      case fB0: (failed B0).
+        have [?] := HB0 _ _ _ _ fB0 dtB0 nB0; subst.
+        case dtB0': det_tree_aux => //=[[[] svB]]//=.
+        have [?] := HA _ _ _ _ fA dtA nA; subst.
+        case dtA': (det_tree_aux _ _ A') => /=[[[] sVA']|]//= _ _.
+        have ? : sVA' = sV2 by admit.
+        subst.
+        rewrite dtB0/=.
+        rewrite dtB0'//=.
+      move: nB0; rewrite next_alt_not_failed//= => -[?]; subst.
+      destruct DA.
+        have {HA}[?] := HA _ _ _ _ fA dtA nA; subst.
+        case: det_tree_aux => /=[[[] sVA']|]//= _.
+        have ? : sVA' = sV2 by admit.
+        subst.
+        rewrite dtB0//.
+      admit.
+    rewrite success_is_ko sA// success_failed//.
+    case dtA: (det_tree_aux _ _ A) => /=[[DA sVA]|]//=.
+    case dtB0: (det_tree_aux _ _ B0) => /=[[DB0 sVB0]|]//=.
+    case dtB: (det_tree_aux _ _ B) => /=[[DB sVB]|]//=.
+    destruct DB0, DB => //= -[?]; subst.
+    case nB: next_alt => [B'|]//=.
+      move=> [<-]{C}/=.
+      rewrite success_is_ko//=dtA/=.
+      have [?] := HB _ _ _ _ fB dtB nB; subst.
+      case dtB': (det_tree_aux _ _ B') => /=[[[] sVB']|]//=.
+      rewrite dtB0/=.
+      by have /=[->] := success_det_tree_next_alt sA dtA.
+    case nA: next_alt => [A'|]//=.
+    case nB0: next_alt => [B0'|]//=.
+    move=> [<-]/={C}.
+    have /=fA' := next_alt_failed nA.
+    destruct DA.
+      have /=[?] := success_det_tree_next_alt sA dtA; subst.
+      rewrite nA => //=.
+      move: fA' => /failed_is_ko kA' dA'.
+      by rewrite is_dead_is_ko in kA'.
+    rewrite failed_is_ko//=.
+    case fB0: (failed B0).
+      have [?] := HB0 _ _ _ _ fB0 dtB0 nB0; subst.
+      by case dtB0': det_tree_aux => //=[[[] svB]]//=.
+    move: nB0; rewrite next_alt_not_failed//= => -[?]; subst.
+    move=> {HB0 HB HA}.
+    case dtA': det_tree_aux => /=[[DA' sVA']|].
+      have ? : sVA' = sV2 by admit.
+      subst.
+      destruct DA'.
+        rewrite (det_tree_aux_func2 dtB0)//=.
+        admit.
+      rewrite dtB0//=.
+      admit.
+    admit. (*should be easy*)
+Admitted. 
+
+Lemma run_is_det {sP A}: 
   check_program sP -> 
     det_tree sP A -> is_det A.
 Proof.
   rewrite/is_det.
-  move=> H1 H2 s s' B []b H3.
-  elim: H3 H2; clear -H1 => //.
-  - move=> s s' A B C b HA -> fA s2.
-    have H := expandedb_next_alt_done H1 fA HA _.
-    have sB := expanded_Done_success u HA.
-    have//:= next_alt_clean_success sB (H s2).
-  - move=> s s' r A B C D b1 b2 b3 HA HB HC IH ? fA s2; subst.
-    apply: IH.
-    apply: expandedb_next_alt_failed H1 fA HA _ HB.
-Qed.
+  move=> ckP + u s s' B n H.
+  elim: H ; clear -ckP => //=.
+  - move=> s1 s2 A B sA _ <-.
+    rewrite /det_tree.
+    case dtA: det_tree_aux => //=[[[] sVA]]// _.
+    by have /=-> := success_det_tree_next_alt sA dtA.
+  - move=> s1 s2 r A B n eA _ dtB dtA.
+    apply: dtB.
+    admit.
+  - move=> s1 s2 r A B n eA _ dtB dtA.
+    apply: dtB.
+    admit.
+  - move=> s1 s2 A B r n fA nA _ dtB dtA.
+    move:dtA; rewrite/det_tree.
+    case dtA: det_tree_aux => /=[[[] svA']|]//= _.
+    apply: dtB.
+    have [_//]:= failed_det_tree_next_alt fA dtA nA.
+  - move=> *; rewrite is_dead_dead//.
+Admitted.
 
 Lemma main {sP p t}:
-  check_program sP -> callable_is_det sP t -> 
+  check_program sP -> det_tree sP (CallS p t) -> 
     is_det ((CallS p t)).
 Proof.
-  move=> H1 fA HA.
-  apply: runb_next_alt H1 _ HA.
-  apply: fA.
+  apply: run_is_det.
 Qed.
 
 Print Assumptions  main.
 
 Section tail_cut.
 
-  Definition tail_cut (r : R) :=
+  (* Definition tail_cut (r : R) :=
   match r.(premises) with [::] => false | x :: xs => last x xs == ACut end.
   
   Definition AllTailCut := (forall pr : program, all tail_cut (rules pr)).
@@ -991,7 +1259,7 @@ Section tail_cut.
   Proof.
     move=> /(cut_in_prem_tail_cut sP).
     apply main.
-  Qed.
+  Qed. *)
 End tail_cut.
 
 Print Assumptions tail_cut_is_det.
